norm checking

proofs/specs/MLDSA_W32_Rep.ec
@@ -1,11 +1,11 @@
-require import AllCore.
+require import AllCore IntDiv List.
 
 from Jasmin require import JWord.
 
 require import GFq Rq VecMat.
 require import Array256.
 
-import CDR Round Zq PolyLVec PolyKVec PolyMat.
+import Parameters CDR Round Zq PolyLVec PolyKVec PolyMat.
 
 (******************************************************)
 (* Representations of polys as 32-bit word arrays     *)
@@ -26,6 +26,17 @@ op poly_srng(bl bh : int, p : poly) = all (fun i => -bl <= crepr i <= bh) p.
 
 op wpoly_urng(b : int, pw : wpoly) = all (fun i => 0 <= W32.to_uint i < b) pw.
 op wpoly_srng(bl bh : int, pw : wpoly) = all (fun i => -bl <= W32.to_sint i <= bh) pw.
+op wpoly_infnorm_lt(b : int, pw : wpoly) = wpoly_srng (b-1) (b-1) pw.
+
+lemma wpoly_infnorm_liftE (b : int) (pw : wpoly) :
+    0 < b <= q %/ 2 =>
+    wpoly_infnorm_lt b pw => infnorm_lt (lifts_wpoly pw) b.
+move => Hb.
+rewrite /wpoly_infnorm_lt /infnorm_lt /wpoly_srng /lifts_wpoly !allP /=.
+move => H j; rewrite mem_iota /= => Hj; have := H j _; 1: smt().
+rewrite mapiE 1:/# /=.
+move => [Hl Hr]; have /# := incoeffK_centered (to_sint pw.[j]) _; 1: smt().
+qed.
 
  
 type wpolylvec = wpoly LArray.t. 
@@ -43,6 +54,46 @@ op polylvec_srng(p : polylvec, bl bh : int) = all (poly_srng bl bh) p.
 
 op wpolylvec_urng(pw : wpolylvec, b : int) = all (wpoly_urng b) pw.
 op wpolylvec_srng(pw : wpolylvec, bl bh : int) = all (wpoly_srng bl bh) pw.
+op wpolylvec_infnorm_lt(b : int, pw : wpolylvec) = wpolylvec_srng pw (b-1) (b-1).
+
+lemma wpolylvec_infnorm_liftE (b : int) (pw : wpolylvec) :
+    0 < b <= q %/ 2 =>
+    wpolylvec_infnorm_lt b pw => PolyLVec.infnorm_lt (lifts_wpolylvec pw) b.
+proof.
+move => Hb.
+rewrite /wpolylvec_infnorm_lt /wpolylvec_srng /polylvec_infnorm_lt /lifts_wpolylvec allP /= => H.
+rewrite /infnorm_lt allP => i; rewrite mem_iota /= => Hi.
+rewrite allP => k; rewrite mem_iota /= => Hk.
+rewrite mapiE 1:/# /= mapiE 1:/# /=.
+have := H i _; 1: smt().
+rewrite /wpoly_srng allP => Hi'.
+have /= := Hi' k _; 1: smt().
+by  have /# := incoeffK_centered (to_sint pw.[i].[k]) _; 1: smt().
+qed.
+
+(* Reverse direction: spec infnorm implies word infnorm, given range ensuring incoeffK_centered applies *)
+lemma wpolylvec_infnorm_unliftE (b bl bh : int) (pw : wpolylvec) :
+    0 < b <= q %/ 2 =>
+    bl + 1 <= q %/ 2 => bh <= q %/ 2 =>
+    wpolylvec_srng pw bl bh =>
+    PolyLVec.infnorm_lt (lifts_wpolylvec pw) b => wpolylvec_infnorm_lt b pw.
+proof.
+move => Hb Hbl Hbh Hrng Hinf.
+rewrite /wpolylvec_infnorm_lt /wpolylvec_srng allP => i  Hi.
+rewrite /wpoly_srng allP => k /= Hk.
+move: Hinf; rewrite /PolyLVec.infnorm_lt /lifts_wpolylvec allP /= => Hinf.
+have /= Hi' := Hinf i _; 1: smt(mem_iota).
+move: Hi'; rewrite allP /= => Hi'.
+have /= Hk' := Hi' k _; 1: smt(mem_iota).
+rewrite mapiE 1:/# /= in Hk'.
+move: Hrng; rewrite /wpolylvec_srng allP => Hrng.
+have /= Hrng_i := Hrng i _; 1: smt().
+move: Hrng_i; rewrite /wpoly_srng allP => /= Hrng_i.
+have /= Hrng_k := Hrng_i k _; 1: smt().
+have := Hk'; rewrite /lifts_wpoly mapiE 1:/# /=.
+by  have/#  := incoeffK_centered (to_sint pw.[i].[k]) _; 1: smt().
+qed.
+
 
 type wpolykvec = wpoly KArray.t. 
 
@@ -59,6 +110,22 @@ op polykvec_srng(p : polykvec, bl bh : int) = all (poly_srng bl bh) p.
 
 op wpolykvec_urng(pw : wpolykvec, b : int) = all (wpoly_urng b) pw.
 op wpolykvec_srng(pw : wpolykvec, bl bh : int) = all (wpoly_srng bl bh) pw.
+op wpolykvec_infnorm(b : int, pw : wpolykvec) = wpolykvec_srng pw (b-1) (b-1).
+
+lemma wpolykvec_infnorm_liftE (b : int) (pw : wpolykvec) :
+    0 < b <= q %/ 2 =>
+    wpolykvec_infnorm b pw => PolyKVec.infnorm (lifts_wpolykvec pw) b.
+proof.
+move => Hb.
+rewrite /wpolykvec_infnorm /wpolykvec_srng /polykvec_infnorm /lifts_wpolykvec allP /= => H.
+rewrite /infnorm allP => i; rewrite mem_iota /= => Hi.
+rewrite allP => k; rewrite mem_iota /= => Hk.
+rewrite mapiE 1:/# /= mapiE 1:/# /=.
+have := H i _; 1: smt().
+rewrite /wpoly_srng allP => Hi'.
+have /= := Hi' k _; 1: smt().
+by  have /# := incoeffK_centered (to_sint pw.[i].[k]) _; 1: smt().
+qed.
 
 type wpolymat = wpoly KLMatrix.t.
 
