proofs/eclib/bindings.ec
@@ -60,7 +60,10 @@ bind circuit
     VPSRLDQ_128 <- "VPSRLDQ_128",
     VPACKUS_8u32 <- "VPACKUS_8u32",
     VPCMPEQ_16u8 <- "VPCMPEQ_16u8",
-    MOVEMASK_16u8 <- "VPMOVMSKB_128"
+    MOVEMASK_16u8 <- "VPMOVMSKB_128",
+    VPCMPGT_8u32 <- "VPCMPGT_8u32",
+    VPABS_8u32 <- "VPABS_8u32",
+    MOVEMASK_8u32 <- "MOVEMASK_8u32"
         from "specs/avx2.spec".
 
 
