proofs/x86-64/avx2/ml_dsa_65/polynomial.ec
@@ -1,0 +1,95 @@
+require import AllCore List IntDiv RealExp.
+
+from Jasmin require import JModel_x86.
+
+from JazzEC require import Ml_dsa_65_avx2 Mldsa_65_prelude.
+
+require import CircuitBindings Bindings.
+
+from Spec require import GFq Rq Parameters MLDSA_W32_Rep Symmetric Serialization.
+
+import CDR Round Zq.
+
+require import XArray256 Array256.
+
+require import WArray1024.
+
+op check_inf_norm_circuit (_a : W32.t Array256.t) (_threshold : int) : bool =
+   all (fun i => (W32.of_int (-_threshold) \slt _a.[i] /\ _a.[i] \slt W32.of_int (_threshold)))  (iotared 0 256).
+
+lemma polynomial____check_infinity_norm_correct (_a : W32.t Array256.t) (_threshold : int) :
+   hoare [ M.polynomial____check_infinity_norm :
+       _threshold = (1 `<<` gamma1m1_bits) - 49 * w1_bits /\
+       polynomial = _a /\ threshold = _threshold /\
+       wpoly_srng (gamma1-1) gamma1 _a
+     ==>
+       (wpoly_infnorm_lt _threshold _a => res = W64.zero) /\
+       (!wpoly_infnorm_lt _threshold _a => res <> W64.zero)
+   ].
+proof.
+rewrite /(`<<`) /=.
+proc => /=.
+seq 2 : (#pre /\ threshold_vector = W256.of_int (524091)).
++ auto => /> *; rewrite /VMOV_64 /= to_uint_eq to_uint_zeroextu256 of_uintK /=.
+  rewrite -(W128.of_uintK 524091); congr; rewrite wordP => i ib.
+  rewrite /pack2_t initiE 1:/# /= get_of_list 1:/# /= of_intE /= bits2wE initiE 1:/# /=.
+  case (i %/ 64 = 0) => ? /=.
+  + rewrite of_intE /= bits2wE initiE 1:/# /=.
+    by rewrite /BitEncoding.BS2Int.int2bs nth_mkseq 1:/# /= nth_mkseq 1:/# /= /#.
+  rewrite /BitEncoding.BS2Int.int2bs nth_mkseq 1:/# /=.
+  rewrite pdiv_small; last by smt().
+  smt(@StdOrder pow2_64).
+  
+proc change ^while.1 : { coefficients <- if (0 <= offset*8 <= 32*256-256)
+                                         then BSWAS_256u32_256.sliceget polynomial (offset*8)
+                                         else get256_direct (WArray1024.init32 (fun i => polynomial.[i])) offset; }.
+                + auto => /> &2.
+                  case (0 <= offset{2} * 8 <= 7936); last by auto.
+                  by move => ?; rewrite BSWAS_256u32_256_slicegetE /#.
+
+wp 7.
+proc change 7 : { zf <- msb_mask = W32.zero; }.
++ by auto => /= &1 &2 ->; rewrite /TEST_32 /rflags_of_bwop /= /ZF_of  /=.
+                  
+unroll for ^while.
+cfold 131.
+wp -1.
+conseq (: polynomial = _a /\ threshold_vector = W256.of_int 524091 /\
+          all (fun i => W32.of_int (-(524288-1)) \sle _a.[i] /\ _a.[i] \sle W32.of_int 524288) (iotared 0 256) ==>
+    zf =  (check_inf_norm_circuit _a 524092)); last 
+     by rewrite  /check_inf_norm_circuit /=; circuit.  
+
+
+(*  Connect circuit form to poly_infnorm spec *)
++ move =>  &1; rewrite iotaredE mldsa65_gamma1 => |>; rewrite /wpoly_srng !allP /= => H.
+  move => x; rewrite mem_iota /= => *; rewrite /(\sle) /= !of_sintK /= /smod /= /#.
+
+move => &hr [[H H1] H2] msbm -> /=; rewrite /wpoly_infnorm /wpoly_srng /check_inf_norm_circuit !allP /SETcc;split;rewrite iotaredE /TEST_32 /= => H3.
++ rewrite ifF /=.
+  + rewrite  /(\slt) /= !of_sintK /= /smod /=.
+    move => x; rewrite mem_iota => ?.
+    move : H3; rewrite /wpoly_infnorm_lt /wpoly_srng allP /= /#.
+  by rewrite to_uint_eq /=.
+    
+rewrite ifT /=.
+  + rewrite  /(\slt) /= !of_sintK /= /smod /=.
+    move : H3; rewrite /wpoly_infnorm_lt /wpoly_srng allP /=;smt(mem_iota).
+  by rewrite to_uint_eq /=.
+qed.
+
+lemma polynomial____check_infinity_norm_ll : islossless M.polynomial____check_infinity_norm.
+proof.
+proc.
+wp;while (0 <= offset <= 1024 /\ offset %% 32 = 0) (1024 - offset); auto => /> /#.
+qed.
+
+lemma polynomial____check_infinity_norm_ph (_a : W32.t Array256.t) (_threshold : int) :
+   phoare [ M.polynomial____check_infinity_norm :
+       _threshold = (1 `<<` gamma1m1_bits) - 49 * w1_bits /\
+       polynomial = _a /\ threshold = _threshold /\
+       wpoly_srng (gamma1-1) gamma1 _a
+     ==>
+       (wpoly_infnorm_lt _threshold _a => res = W64.zero) /\
+       (!wpoly_infnorm_lt _threshold _a => res <> W64.zero)
+   ] = 1%r
+ by  conseq polynomial____check_infinity_norm_ll (polynomial____check_infinity_norm_correct _a _threshold).
